LinkedJournal InternalJournalMarshal works; added diskview framing argument

Splinter/Journal/LinkedJournal.i.dfy
@@ -9,13 +9,83 @@ module LinkedJournal {
   import opened MsgHistoryMod
   import opened LSNMod
   import opened Sequences
+  import opened JournalLabels
   import PagedJournal
 
   type Address(!new, ==)
   type Pointer = Option<Address>
 
+  type Ranking = map<Address, nat>
+
   // TODO(robj): where does this go?
+  // The DiskView in this module is a tightly-populated mapping:
+  // every record the journal needs is present in the mapping,
+  // and every address is "important" to the journal.
   datatype DiskView = DiskView(entries: map<Address, JournalRecord>) {
+    predicate EntriesWF()
+    {
+      (forall addr | addr in entries :: entries[addr].WF())
+    }
+
+    predicate NondanglingPointer(ptr: Pointer)
+    {
+      ptr.Some? ==> ptr.value in entries
+    }
+
+    predicate NondanglingPointers()
+    {
+      (forall addr | addr in entries :: NondanglingPointer(entries[addr].priorRec))
+    }
+
+    predicate WF()
+    {
+      && EntriesWF()
+      && NondanglingPointers()
+    }
+
+    predicate PointersRespectRank(ranking: Ranking)
+      requires WF()
+    {
+      && ranking.Keys == entries.Keys
+      && (forall address | address in entries && entries[address].priorRec.Some? ::
+          && ranking[entries[address].priorRec.value] < ranking[address]
+         )
+    }
+
+    predicate Acyclic()
+      requires WF()
+    {
+      && exists ranking :: PointersRespectRank(ranking)
+    }
+
+    function TheRanking() : Ranking
+      requires WF()
+      requires Acyclic()
+    {
+      // Make CHOOSE deterministic as Leslie and Hilbert intended
+      var ranking :| PointersRespectRank(ranking); ranking
+    }
+
+    function RankedIPtr(ptr: Pointer, ranking: Ranking) : Option<PagedJournal.JournalRecord>
+      requires WF()
+      requires NondanglingPointer(ptr)
+      requires PointersRespectRank(ranking)
+      decreases if ptr.Some? then ranking[ptr.value] else -1 // I can't believe this works, Rustan!
+    {
+      if ptr.None?
+      then None
+      else
+        var jr := entries[ptr.value];
+        Some(PagedJournal.JournalRecord(jr.messageSeq, RankedIPtr(jr.priorRec, ranking)))
+    }
+
+    function IPtr(ptr: Pointer) : Option<PagedJournal.JournalRecord>
+      requires WF()
+      requires Acyclic()
+      requires NondanglingPointer(ptr)
+    {
+      RankedIPtr(ptr, TheRanking())
+    }
   }
 
   datatype JournalRecord = JournalRecord(messageSeq: MsgHistory, priorRec: Pointer)
@@ -25,15 +95,66 @@ module LinkedJournal {
       messageSeq.WF()
     }
   }
-    
+
   datatype TruncatedJournal = TruncatedJournal(
     boundaryLSN : LSN,  // exclusive: lsns <= boundaryLSN are discarded
     freshestRec: Pointer,
-    cacheView: DiskView)
+    diskView: DiskView)
+  {
+    predicate WF() {
+      && diskView.WF()
+      && diskView.NondanglingPointer(freshestRec)
+    }
+
+    function SeqStart() : LSN
+    {
+      boundaryLSN
+    }
+
+    function SeqEnd() : LSN
+      requires WF()
+    {
+      if freshestRec.None?  // normal case with empty TJ
+      then boundaryLSN
+      else diskView.entries[freshestRec.value].messageSeq.seqEnd
+    }
+
+    // TODO(jonh): this function doesn't yet correctly maintain the "DiskView
+    // tightness" property; it leaks pages. We'll probably need a receipt to locate
+    // the subset of addresses we want to keep.
+    function DiscardOld(lsn: LSN) : (out:TruncatedJournal)
+      requires WF()
+    {
+      if freshestRec.None? || lsn == diskView.entries[freshestRec.value].messageSeq.seqEnd
+      then TruncatedJournal(lsn, None, diskView)
+      else TruncatedJournal(lsn, freshestRec, diskView)
+    }
+
+    function AppendRecord(addr: Address, msgs: MsgHistory) : (out: TruncatedJournal)
+      requires addr !in diskView.entries
+    {
+      this.(
+        diskView := diskView.(entries := diskView.entries[addr := JournalRecord(msgs, freshestRec)]),
+        freshestRec := Some(addr))
+    }
+
+    function I() : PagedJournal.TruncatedJournal
+      requires WF()
+      requires diskView.Acyclic()
+    {
+      PagedJournal.TruncatedJournal(boundaryLSN, diskView.IPtr(freshestRec))
+    }
+
+    predicate Decodable()
+    {
+      && WF()
+      && diskView.Acyclic()
+      && I().WF()
+    }
+  }
 
   function Mkfs() : (out:TruncatedJournal)
   {
-    // TODO(jonh): Just making up DiskViews seems like trouble for lower in the stack.
     TruncatedJournal(0, None, DiskView(map[]))
   }
 
@@ -47,55 +168,106 @@ module LinkedJournal {
       && unmarshalledTail.WF()
       && truncatedJournal.SeqEnd() == unmarshalledTail.seqStart
     }
+
+    function SeqStart() : LSN
+    {
+      truncatedJournal.SeqStart()
+    }
+
+    function SeqEnd() : LSN
+      requires WF()
+    {
+      unmarshalledTail.seqEnd
+    }
+
+    predicate UnusedAddr(addr: Address)
+    {
+      // TODO reaching into truncatedJournal to find the diskView feels skeezy
+      addr !in truncatedJournal.diskView.entries
+    }
   }
 
-  predicate Put(v: Variables, v': Variables, msgs: MsgHistory)
+  // NB We need both rank and receipts to concisely write this predicate, which is why they
+  // get defined here in the state machine instead of deferred to the refinement module.
+  predicate ReadForRecovery(v: Variables, v': Variables, lbl: TransitionLabel, receiptIndex: nat)
   {
+    && lbl.ReadForRecoveryLabel?
+    && lbl.messages.WF()
     && v.WF()
-    && v'.WF()
-    && msgs.WF()
-    && (v.SeqEnd().None? || msgs.EmptyHistory? || msgs.seqStart == v.SeqEnd().value)  // CanFollow, but without interpreting this.
-    && v' == v.(unmarshalledTail := v.unmarshalledTail.Concat(msgs))
+    && v.truncatedJournal.Decodable()
+    && var pagedTJ := v.truncatedJournal.I();
+    && pagedTJ.IncludesSubseqAt(lbl.messages, receiptIndex)
+    && v' == v
   }
 
-  predicate DiscardOld(v: Variables, v': Variables, lsn: LSN)
+  predicate FreezeForCommit(v: Variables, v': Variables, lbl: TransitionLabel, keepReceiptLines: nat)
   {
     && v.WF()
-    && v'.WF()
-    && (if v.Empty() then true else v.SeqStart() <= lsn <= v.SeqEnd().value)
-    && (if v.unmarshalledTail.MsgHistory? && v.unmarshalledTail.seqStart <= lsn
-        then v' == Variables(Mkfs(), v.unmarshalledTail.DiscardOld(lsn))
-        else v' == v.(truncatedJournal := v.truncatedJournal.DiscardOld(lsn))
+    && v.truncatedJournal.Decodable()
+    && var pagedTJ := v.truncatedJournal.I();
+    && pagedTJ.FreezeForCommit(lbl, keepReceiptLines)
+    && v' == v
+  }
+
+  // rename to match lbl QueryEndLsnLabel
+  predicate ObserveFreshJournal(v: Variables, v': Variables, lbl: TransitionLabel)
+  {
+    && lbl.QueryEndLsnLabel?
+    && v.WF()
+    && lbl.endLsn == v.SeqEnd()
+    && v' == v
+  }
+
+  predicate Put(v: Variables, v': Variables, lbl: TransitionLabel)
+  {
+    && lbl.PutLabel?
+    && lbl.messages.WF()
+    && v.WF()
+    && lbl.messages.seqStart == v.SeqEnd()
+    && v' == v.(unmarshalledTail := v.unmarshalledTail.Concat(lbl.messages))
+  }
+
+  predicate DiscardOld(v: Variables, v': Variables, lbl: TransitionLabel)
+  {
+    // diskView not tightened here
+    && lbl.DiscardOldLabel?
+    && v.WF()
+    && lbl.requireEnd == v.SeqEnd()
+    && v.SeqStart() <= lbl.startLsn <= v.SeqEnd()
+    && (if v.unmarshalledTail.seqStart <= lbl.startLsn
+        then v' == Variables(Mkfs(), v.unmarshalledTail.DiscardOld(lbl.startLsn))
+        else v' == v.(truncatedJournal := v.truncatedJournal.DiscardOld(lbl.startLsn))
        )
   }
 
-  predicate JournalMarshal(v: Variables, v': Variables, cut: LSN)
+  predicate InternalJournalMarshal(v: Variables, v': Variables, lbl: TransitionLabel, cut: LSN, addr: Address)
   {
+    && lbl.InternalLabel?
     && v.WF()
-    && v'.WF()
-    && v.unmarshalledTail.MsgHistory?
     && v.unmarshalledTail.seqStart < cut // Can't marshall nothing.
     && v.unmarshalledTail.CanDiscardTo(cut)
+    && v.UnusedAddr(addr)
     && var marshalledMsgs := v.unmarshalledTail.DiscardRecent(cut);
     && v' == Variables(
-      v.truncatedJournal.AppendRecord(marshalledMsgs),
+      v.truncatedJournal.AppendRecord(addr, marshalledMsgs),
       v.unmarshalledTail.DiscardOld(cut))
   }
 
-  predicate Init(v: Variables)
+  predicate Init(v: Variables, tj: TruncatedJournal)
   {
-    && v == Variables(Mkfs(), EmptyHistory)
+    && tj.Decodable() // An invariant carried by CoordinationSystem from FreezeForCommit, past a crash, back here
+    && v == Variables(tj, EmptyHistoryAt(tj.SeqEnd()))
   }
 
   datatype Step =
       ReadForRecoveryStep(receiptIndex: nat)
     | FreezeForCommitStep(keepReceiptLines: nat)
     | ObserveFreshJournalLabel()
-    | PutStep(msgs: MsgHistory)
-    | DiscardOldStep(lsn: LSN)
-    | InternalJournalMarshalStep(cut: LSN)
+    | PutStep()
+    | DiscardOldStep()
+    | InternalJournalMarshalStep(cut: LSN, addr: Address)
 
-  predicate NextStep(v: Variables, v': Variables, step: Step)
+  predicate NextStep(v: Variables, v': Variables, lbl: TransitionLabel, step: Step)
   {
     match step {
       case ReadForRecoveryStep(receiptIndex) => ReadForRecovery(v, v', lbl, receiptIndex)
@@ -103,7 +275,11 @@ module LinkedJournal {
       case ObserveFreshJournalLabel() => ObserveFreshJournal(v, v', lbl)
       case PutStep() => Put(v, v', lbl)
       case DiscardOldStep() => DiscardOld(v, v', lbl)
-      case InternalJournalMarshalStep(cut) => InternalJournalMarshal(v, v', lbl, cut)
+      case InternalJournalMarshalStep(cut, addr) => InternalJournalMarshal(v, v', lbl, cut, addr)
     }
+  }
+
+  predicate Next(v: Variables, v': Variables, lbl: TransitionLabel) {
+    exists step: Step :: NextStep(v, v', lbl, step)
   }
 }
