Splinter/Journal/LinkedJournalRefinement.i.dfy
@@ -1,0 +1,146 @@
+// Copyright 2018-2021 VMware, Inc., Microsoft Inc., Carnegie Mellon University, ETH Zurich, and University of Washington
+// SPDX-License-Identifier: BSD-2-Clause
+
+include "LinkedJournal.i.dfy"
+include "PagedJournalRefinement.i.dfy"
+
+module LinkedJournalRefinement
+// TODO refines RefinementObligation(JournalLabels, PagedJournal)
+{
+  import opened Options
+  import opened MsgHistoryMod
+  import opened LSNMod
+  import opened JournalLabels
+  import PagedJournal
+  import PagedJournalRefinement
+  import opened LinkedJournal
+
+  predicate Inv(v: Variables)
+  {
+    && v.WF()
+    && v.truncatedJournal.Decodable()
+  }
+  
+  function I(v: Variables) : PagedJournal.Variables
+    requires v.WF()
+    requires v.truncatedJournal.diskView.Acyclic()
+  {
+    PagedJournal.Variables(v.truncatedJournal.I(), v.unmarshalledTail)
+  }
+
+  // TODO(robj): move this to maps
+  predicate Submap<K,V>(a: map<K,V>, b: map<K,V>)
+  {
+    forall k | k in a :: k in b && a[k] == b[k]
+  }
+
+  lemma RankedIPtrFraming(dv1: DiskView, dv2: DiskView, r1: Ranking, r2: Ranking, ptr: Pointer)
+    requires dv1.WF() && dv1.Acyclic() && dv1.PointersRespectRank(r1)
+    requires dv2.WF() && dv2.Acyclic() && dv2.PointersRespectRank(r2)
+    requires dv1.NondanglingPointer(ptr)
+    requires Submap(dv1.entries, dv2.entries)
+    ensures dv1.RankedIPtr(ptr, r1) == dv2.RankedIPtr(ptr, r2)
+    decreases if ptr.Some? then r1[ptr.value] else -1
+  {
+    if ptr != None {
+      RankedIPtrFraming(dv1, dv2, r1, r2, dv1.entries[ptr.value].priorRec);
+    }
+  }
+
+  lemma IPtrFraming(dv1: DiskView, dv2: DiskView, ptr: Pointer)
+    requires dv1.WF() && dv1.Acyclic()
+    requires dv2.WF() && dv2.Acyclic()
+    requires dv1.NondanglingPointer(ptr)
+    requires Submap(dv1.entries, dv2.entries)
+    ensures dv1.IPtr(ptr) == dv2.IPtr(ptr)
+  {
+    RankedIPtrFraming(dv1, dv2, dv1.TheRanking(), dv2.TheRanking(), ptr);
+  }
+
+  //////////////////////////////////////////////////////////////////////////////
+  // non-state-machine function & predicate refinement lemmas
+
+  lemma MkfsRefines()
+    ensures Mkfs().diskView.Acyclic()
+    ensures Mkfs().I() == PagedJournal.Mkfs()
+  {
+    assert Mkfs().diskView.PointersRespectRank(map[]);  // witness to exists ranking
+  }
+
+  //////////////////////////////////////////////////////////////////////////////
+  // State machine refinement
+
+  lemma InvInit(v: Variables, tj: TruncatedJournal)
+    requires Init(v, tj)
+    ensures Inv(v)
+  {
+  }
+
+  lemma InvNext(v: Variables, v': Variables, lbl: TransitionLabel)
+    requires Inv(v)
+    requires Next(v, v', lbl)
+    ensures Inv(v')
+  {
+    var step: Step :| NextStep(v, v', lbl, step);
+    if step.ReadForRecoveryStep? {
+      assert Inv(v');
+    } else if step.FreezeForCommitStep? {
+      assert Inv(v');
+    } else if step.ObserveFreshJournalLabel? {
+      assert Inv(v');
+    } else if step.PutStep? {
+      assert Inv(v');
+    } else if step.DiscardOldStep? {
+      assume false;
+      assert PagedJournal.DiscardOld(I(v), I(v'), lbl);
+      assert v'.WF();
+      assert v'.truncatedJournal.Decodable();
+      assert Inv(v');
+    } else if step.InternalJournalMarshalStep? {
+      // Witness new rank
+      var rank :| v.truncatedJournal.diskView.PointersRespectRank(rank);
+      var rank' := rank[step.addr :=
+          if v.truncatedJournal.freshestRec.None? then 0
+          else rank[v.truncatedJournal.freshestRec.value]+1];
+      assert v'.truncatedJournal.diskView.PointersRespectRank(rank');
+
+      IPtrFraming(v.truncatedJournal.diskView, v'.truncatedJournal.diskView, v.truncatedJournal.freshestRec);
+      assert Inv(v');
+    } else {
+      assert false;
+    }
+  }
+
+  lemma InitRefines(v: Variables, tj: TruncatedJournal)
+    requires Init(v, tj)
+    ensures PagedJournal.Init(I(v), tj.I())
+  {
+  }
+
+  lemma NextRefines(v: Variables, v': Variables, lbl: TransitionLabel)
+    requires Inv(v)
+    requires Next(v, v', lbl)
+    ensures v'.WF()
+    ensures Inv(v')
+    ensures PagedJournal.Next(I(v), I(v'), lbl)
+  {
+    assume false;   // TODO
+    var step: Step :| NextStep(v, v', lbl, step);
+    if step.ReadForRecoveryStep? {
+      assert PagedJournal.Next(I(v), I(v'), lbl);
+    } else if step.FreezeForCommitStep? {
+      assert PagedJournal.Next(I(v), I(v'), lbl);
+    } else if step.ObserveFreshJournalLabel? {
+      assert PagedJournal.Next(I(v), I(v'), lbl);
+    } else if step.PutStep? {
+      assert PagedJournal.Next(I(v), I(v'), lbl);
+    } else if step.DiscardOldStep? {
+      assert PagedJournal.Next(I(v), I(v'), lbl);
+    } else if step.InternalJournalMarshalStep? {
+      assert PagedJournal.Next(I(v), I(v'), lbl);
+    } else {
+      assert false;
+    }
+  }
+}
+
